edits on libs

specs/Spec.SHA3.Constants.fst
@@ -3,25 +3,24 @@ module Spec.SHA3.Constants
 open Lib.IntTypes
 
 #reset-options "--z3rlimit 50 --max_fuel 0 --max_ifuel 0"
+let rotc_t = rotval U64
 
-let rotc_t = x:size_t{0 < uint_v x && uint_v x < 64}
-
-unfold let rotc_list: list rotc_t =
-  [size 1; size 3; size 6; size 10; size 15; size 21; size 28; size 36;
-   size 45; size 55; size 2; size 14; size 27; size 41; size 56; size 8;
-   size 25; size 43; size 62; size 18; size 39; size 61; size 20; size 44]
+unfold let rotc_list:  list rotc_t =
+  [1ul; 3ul; 6ul; 10ul; 15ul; 21ul; 28ul; 36ul;
+   45ul; 55ul; 2ul; 14ul; 27ul; 41ul; 56ul; 8ul;
+   25ul; 43ul; 62ul; 18ul; 39ul; 61ul; 20ul; 44ul]
 
 let piln_t = x:size_t{size_v x < 25}
 
 unfold let piln_list: list piln_t =
-  [size 10; size 7; size 11; size 17; size 18; size 3; size 5; size 16;
-   size 8; size 21; size 24; size 4; size 15; size 23; size 19; size 13;
-   size 12; size 2; size 20; size 14; size 22; size 9; size 6; size 1]
+  [10ul; 7ul; 11ul; 17ul; 18ul; 3ul; 5ul; 16ul;
+   8ul; 21ul; 24ul; 4ul; 15ul; 23ul; 19ul; 13ul;
+   12ul; 2ul; 20ul; 14ul; 22ul; 9ul; 6ul; 1ul]
 
-unfold let rndc_list: list uint64 =
-  [u64 0x0000000000000001; u64 0x0000000000008082; u64 0x800000000000808a; u64 0x8000000080008000;
-   u64 0x000000000000808b; u64 0x0000000080000001; u64 0x8000000080008081; u64 0x8000000000008009;
-   u64 0x000000000000008a; u64 0x0000000000000088; u64 0x0000000080008009; u64 0x000000008000000a;
-   u64 0x000000008000808b; u64 0x800000000000008b; u64 0x8000000000008089; u64 0x8000000000008003;
-   u64 0x8000000000008002; u64 0x8000000000000080; u64 0x000000000000800a; u64 0x800000008000000a;
-   u64 0x8000000080008081; u64 0x8000000000008080; u64 0x0000000080000001; u64 0x8000000080008008]
+unfold let rndc_list: list (uint_t U64 PUB) =
+  [0x0000000000000001uL; 0x0000000000008082uL; 0x800000000000808auL; 0x8000000080008000uL;
+   0x000000000000808buL; 0x0000000080000001uL; 0x8000000080008081uL; 0x8000000000008009uL;
+   0x000000000000008auL; 0x0000000000000088uL; 0x0000000080008009uL; 0x000000008000000auL;
+   0x000000008000808buL; 0x800000000000008buL; 0x8000000000008089uL; 0x8000000000008003uL;
+   0x8000000000008002uL; 0x8000000000000080uL; 0x000000000000800auL; 0x800000008000000auL;
+   0x8000000080008081uL; 0x8000000000008080uL; 0x0000000080000001uL; 0x8000000080008008uL]
